UnitTest/IR/Operation.lean
@@ -1,0 +1,34 @@
+import Veir.IR.Basic
+import Veir.Parser.MlirParser
+
+open Veir
+open Veir.Parser
+
+private def parse (s : String) : OperationPtr × IRContext OpCode :=
+  match WfIRContext.create OpCode with
+  | none => panic! "failed to create IR context"
+  | some (ctx, _) =>
+    match ParserState.fromInput s.toByteArray with
+    | .error _ => panic! "lex error"
+    | .ok parser =>
+      match (parseOp none).run (MlirParserState.fromContext ctx) parser with
+      | .error _ => panic! "parse error"
+      | .ok (op, state, _) => (op, state.ctx.raw)
+
+private def noRegions := parse r#""arith.muli"() : () -> ()"#
+#guard noRegions.1.getNumRegions! noRegions.2 == 0
+
+private def oneRegion := parse r#""arith.addi"() ({
+  "arith.muli"() : () -> ()
+}) : () -> ()"#
+#guard oneRegion.1.getNumRegions! oneRegion.2 == 1
+
+private def twoRegions := parse r#""arith.addi"() ({
+  "arith.muli"() : () -> ()
+}, {
+  "arith.muli"() : () -> ()
+}) : () -> ()"#
+#guard twoRegions.1.getNumRegions! twoRegions.2 == 2
+#guard (twoRegions.1.getRegions! twoRegions.2).size == twoRegions.1.getNumRegions! twoRegions.2
+#guard (twoRegions.1.getRegions! twoRegions.2)[0]! == twoRegions.1.getRegion! twoRegions.2 0
+#guard (twoRegions.1.getRegions! twoRegions.2)[1]! == twoRegions.1.getRegion! twoRegions.2 1
